* Boolean Algebra
  - Define   
    Boolean Algebra is a group including value and its operators,
    $$(\{0, 1\}, \neg, \wedge, \vee)$$

    The value of boolean algebra belongs to $\{\text{true}, \text{false}\}$, usually denoted $\{1, 0\}$.

    The basic operations of boolean algebra include $\neg, \wedge, \vee$.
    - NOT $\neg$  
      NOT is a unary operator.
      |$a$|$\neg a$|
      |---|---|
      | 0 | 0 |
      | 1 | 1 |
      |||

    - AND $\wedge$, OR $\vee$  
      AND, OR are two binary operators.  
      |$a$|$b$|$a \wedge b$|$a \vee b$|
      |:---:|:---:|:---:|:---:|
      | 0 | 0 | 0 | 0 | 
      | 0 | 1 | 0 | 1 | 
      | 1 | 0 | 0 | 1 | 
      | 1 | 1 | 1 | 1 | 
      |||

  - Property
    - |
      - $a \wedge b = b \wedge a$
      - $a \vee b = b \vee a$
      - $(a \wedge b) \wedge c = a \wedge (b \wedge c)$
      - $(a \vee b) \vee c = a \vee (b \vee c)$
      - $\neg(a \wedge b) = \neg a \vee \neg b$
      - $\neg(a \vee b) = \neg a \wedge \neg b$
      - $a \wedge (a \vee b) = a$
      - $a \vee (a \wedge b) = a$
      - $a \wedge (b \vee c) = (a \wedge b) \vee (a \wedge c)$
      - $a \vee (b \wedge c) = (a \vee b) \wedge (a \vee c)$

    * XOR & XNOR
      - Define   
        XOR $\oplus$, XNOR $\odot$ are two binary operators.  
        |$a$|$b$|$a \oplus b$|$a \odot b$|
        |:---:|:---:|:---:|:---:|
        | 0 | 0 | 0 | 1 | 
        | 0 | 1 | 1 | 0 | 
        | 1 | 0 | 1 | 0 | 
        | 1 | 1 | 0 | 1 | 
        |||
        $$a \oplus b = \neg(a \odot b)$$
        $$a \oplus b = (a \wedge \neg b) \vee (\neg a \wedge b)$$

      - Property
        - $x \oplus 0 = x$
        - $x \oplus 1 = \neg x$
        - $x \oplus \neg x = 1$
        - $x \oplus x = 0$
        - $(a \oplus b) \oplus c = a \oplus (b \oplus c)$

    - |
      |$f(0, 0)$|$f(0, 1) = f(1, 0)$|$f(1, 1)$|operator|
      |:---:|:---:|:---:|:---:|
      | 0 | 0 | 0 | $a \wedge 0$ |
      | 0 | 0 | 1 | $a \wedge b$ |
      | 0 | 1 | 0 | $a \oplus b = (a \wedge \neg b) \vee (\neg a \wedge b)$ |
      | 0 | 1 | 1 | $a \vee b$ |
      | 1 | 0 | 0 | $\neg(a \vee b)$ |
      | 1 | 0 | 1 | $a \odot b = (a \vee \neg b) \wedge (\neg a \vee b)$ |
      | 1 | 1 | 0 | $\neg(a \wedge b)$ |
      | 1 | 1 | 1 | $a \vee 0$ |
      |||||